feat: support umod in bv_decide (#5652)

src/Std/Tactic/BVDecide/Bitblast/BVExpr/Basic.lean
@@ -69,6 +69,10 @@ inductive BVBinOp where
   Unsigned division.
   -/
   | udiv
+  /--
+  Unsigned modulo.
+  -/
+  | umod
 
 namespace BVBinOp
 
@@ -79,6 +83,7 @@ def toString : BVBinOp → String
   | add => "+"
   | mul => "*"
   | udiv => "/ᵤ"
+  | umod => "%ᵤ"
 
 instance : ToString BVBinOp := ⟨toString⟩
 
@@ -92,6 +97,7 @@ def eval : BVBinOp → (BitVec w → BitVec w → BitVec w)
   | add => (· + ·)
   | mul => (· * ·)
   | udiv => (· / ·)
+  | umod => (· % · )
 
 @[simp] theorem eval_and : eval .and = ((· &&& ·) : BitVec w → BitVec w → BitVec w) := by rfl
 @[simp] theorem eval_or : eval .or = ((· ||| ·) : BitVec w → BitVec w → BitVec w) := by rfl
@@ -99,6 +105,7 @@ def eval : BVBinOp → (BitVec w → BitVec w → BitVec w)
 @[simp] theorem eval_add : eval .add = ((· + ·) : BitVec w → BitVec w → BitVec w) := by rfl
 @[simp] theorem eval_mul : eval .mul = ((· * ·) : BitVec w → BitVec w → BitVec w) := by rfl
 @[simp] theorem eval_udiv : eval .udiv = ((· / ·) : BitVec w → BitVec w → BitVec w) := by rfl
+@[simp] theorem eval_umod : eval .umod = ((· % ·) : BitVec w → BitVec w → BitVec w) := by rfl
 
 end BVBinOp
 
